Revise the semantics upto the progress lemma

src/lang/Commit.v
@@ -23,7 +23,7 @@ Module Commit <: JoinableType.
   }.
   Definition t := t_.
 
-  Definition elt: t := mk (LocFun.init Capability.elt) Capability.elt Capability.elt.
+  Definition bot: t := mk (LocFun.init Capability.bot) Capability.bot Capability.bot.
 
   Inductive wf (commit:t): Prop :=
   | wf_intro
@@ -119,26 +119,30 @@ Module Commit <: JoinableType.
   Inductive readable
             (commit1:t) (loc:Loc.t) (ts:Time.t) (released:Capability.t) (ord:Ordering.t): Prop :=
   | readable_intro
-      (TS: Time.le (commit1.(cur).(Capability.rw) loc) ts)
+      (UR: Time.le (commit1.(cur).(Capability.ur) loc) ts)
+      (RW: Ordering.le Ordering.relaxed ord ->
+           Time.le (commit1.(cur).(Capability.rw) loc) ts)
       (SC: Ordering.le Ordering.seqcst ord ->
            Time.le (commit1.(cur).(Capability.sc) loc) ts /\
            Time.le (released.(Capability.sc) loc) ts)
   .
 
-  Definition read
+  Definition read_commit
              (commit1:t) (loc:Loc.t) (ts:Time.t) (released:Capability.t) (ord:Ordering.t): t :=
     mk commit1.(rel)
-       (Capability.join_if
-          (Ordering.le Ordering.acqrel ord)
-          released
-          (Capability.incr_rw loc ts commit1.(cur)))
-       (Capability.join_if
-          (Ordering.le Ordering.relaxed ord)
-          released
-          (Capability.incr_rw loc ts commit1.(acq))).
+       (Capability.join
+          (Capability.join
+             commit1.(cur)
+             (Capability.singleton_rw loc ts))
+          (if Ordering.le Ordering.acqrel ord then released else Capability.bot))
+       (Capability.join
+          (Capability.join
+             commit1.(acq)
+             (Capability.singleton_rw loc ts))
+          (if Ordering.le Ordering.relaxed ord then released else Capability.bot)).
 
   Inductive writable
-            (commit1:t) (sc1:TimeMap.t) (loc:Loc.t) (ts:Time.t) (released:Capability.t) (ord:Ordering.t): Prop :=
+            (commit1:t) (sc1:TimeMap.t) (loc:Loc.t) (ts:Time.t) (ord:Ordering.t): Prop :=
   | writable_intro
       (TS: Time.lt (commit1.(cur).(Capability.rw) loc) ts)
       (SC: Ordering.le Ordering.seqcst ord ->
@@ -146,494 +150,307 @@ Module Commit <: JoinableType.
            Time.lt (sc1 loc) ts)
   .
 
-  Definition write
-             (commit1:t) (loc:Loc.t) (ts:Time.t) (ord:Ordering.t): Capability.t * t * TimeMap.t :=
-    let cur := Capability.join_if
-                 (Ordering.le Ordering.seqcst ord)
-                 
-                 (Capability.incr_ur loc ts commit.(Commit.cur))
+  Definition write_commit
+             (commit1:t) (sc1:TimeMap.t) (loc:Loc.t) (ts:Time.t) (ord:Ordering.t): t :=
+    let cur2 := Capability.join
+                  (Capability.join
+                     commit1.(Commit.cur)
+                     (Capability.singleton_ur loc ts))
+                  (if Ordering.le Ordering.seqcst ord then Capability.mk TimeMap.bot TimeMap.bot sc1 else Capability.bot)
     in
+    let acq2 := Capability.join
+                  (Capability.join
+                     commit1.(Commit.acq)
+                     (Capability.singleton_ur loc ts))
+                  (if Ordering.le Ordering.seqcst ord then Capability.mk TimeMap.bot TimeMap.bot sc1 else Capability.bot)
+    in
+    let rel2 := LocFun.add
+                  loc
+                  (Capability.join
+                     (commit1.(Commit.rel) loc)
+                     (if Ordering.le Ordering.acqrel ord then cur2 else Capability.bot))
+                  commit1.(Commit.rel)
+    in
+    Commit.mk rel2 cur2 acq2.
 
-Capability.join
-                 Capability.join released ()
+  Definition write_sc
+             (sc1:TimeMap.t) (loc:Loc.t) (ts:Time.t) (ord:Ordering.t): TimeMap.t :=
+    TimeMap.join
+      sc1
+      (if Ordering.le Ordering.seqcst ord then TimeMap.singleton loc ts else TimeMap.bot).
 
-            (commit2:t): Prop :=
+  Definition read_fence_commit
+             (commit1:t) (ord:Ordering.t): t :=
+    Commit.mk commit1.(Commit.rel)
+              (if Ordering.le Ordering.acqrel ord
+               then commit1.(Commit.acq)
+               else commit1.(Commit.cur))
+              commit1.(Commit.acq).
 
-             loc ts released commit: Commit.t :=
-    (Commit.mk (LocFun.add loc released commit.(Commit.rel))
-               (Capability.join released (Capability.incr_ur loc ts commit.(Commit.cur)))
-               (Capability.join released (Capability.incr_ur loc ts commit.(Commit.acq)))).
-  
+  Definition write_fence_sc
+             (commit1:t) (sc1:TimeMap.t) (ord:Ordering.t): TimeMap.t :=
+    TimeMap.join
+      sc1
+      (if Ordering.le Ordering.seqcst ord then commit1.(Commit.cur).(Capability.sc) else TimeMap.bot).
 
-  Inductive write
-            (commit1:t) (loc:Loc.t) (ts:Time.t) (released:Capability.t) (ord:Ordering.t)
-            (commit2:t): Prop :=
-  | write_intro
-      (MON: le commit1 commit2)
-      (REL: Time.le (released.(Capability.rw) loc) ts)
-      (RW1: Time.lt (commit1.(cur).(Capability.rw) loc) ts)
-      (RW2: Time.le ts (commit2.(cur).(Capability.ur) loc))
-      (REL1: Capability.le (commit1.(Commit.rel) loc) released)
-      (REL2: Capability.le released (commit2.(Commit.rel) loc))
-      (RA: Ordering.le Ordering.acqrel ord ->
-           Capability.le commit1.(Commit.cur) released /\
-           Time.le ts (released.(Capability.rw) loc))
-      (WF_REL: Capability.wf released)
-      (WF: Commit.wf commit2)
-  .
-
-  Inductive read_fence
-            (commit1:t) (ord:Ordering.t)
-            (commit2:t): Prop :=
-  | read_fence_intro
-      (MON: le commit1 commit2)
-      (RA: Ordering.le Ordering.acqrel ord ->
-           Capability.le commit1.(Commit.acq) commit2.(Commit.cur))
-      (WF: Commit.wf commit2)
-  .
-
-  Inductive write_fence
-            (commit1:t) (ord:Ordering.t)
-            (commit2:t): Prop :=
-  | write_fence_intro
-      (MON: le commit1 commit2)
-      (RA: Ordering.le Ordering.acqrel ord ->
-           forall loc, Capability.le commit1.(Commit.cur) (commit2.(Commit.rel) loc))
-      (WF: Commit.wf commit2)
-  .
+  Definition write_fence_commit
+             (commit1:t) (sc1:TimeMap.t) (ord:Ordering.t): t :=
+    let sc2 := write_fence_sc commit1 sc1 ord in
+    let cur2 := Capability.join
+                  commit1.(Commit.cur)
+                  (if Ordering.le Ordering.seqcst ord then Capability.mk sc2 sc2 sc2 else Capability.bot)
+    in
+    let acq2 := Capability.join
+                  commit1.(Commit.acq)
+                  (if Ordering.le Ordering.seqcst ord then Capability.mk sc2 sc2 sc2 else Capability.bot)
+    in
+    let rel2 := fun l =>
+                  Capability.join
+                    (commit1.(Commit.rel) l)
+                    (if Ordering.le Ordering.acqrel ord then cur2 else Capability.bot)
+    in
+    Commit.mk rel2 cur2 acq2.
 End Commit.
 
 Module CommitFacts.
   Ltac tac :=
     repeat
       (try match goal with
-           | [|- Capability.le (Capability.join _ _) _] =>
-             apply Capability.join_spec
-           | [|- Capability.le (Capability.incr_ur _ _ _) _] =>
-             apply Capability.incr_ur_spec
-           | [|- Capability.le (Capability.incr_rw _ _ _) _] =>
-             apply Capability.incr_rw_spec
-
-           | [|- TimeMap.le (TimeMap.incr _ _ _) _] =>
-             apply TimeMap.incr_spec
-           | [|- Capability.le ?s (Capability.incr_ur _ _ ?s)] =>
-             apply Capability.incr_ur_le
-           | [|- Capability.le ?s (Capability.incr_rw _ _ ?s)] =>
-             apply Capability.incr_rw_le
-
+           | [|- Capability.le ?s ?s] =>
+             refl
+           | [|- TimeMap.le ?s ?s] =>
+             refl
+           | [|- Capability.le Capability.bot ?s] =>
+             apply Capability.bot_spec
            | [|- Capability.le ?s (Capability.join _ ?s)] =>
              apply Capability.join_r
            | [|- Capability.le ?s (Capability.join ?s _)] =>
              apply Capability.join_l
+           | [|- TimeMap.le ?s (TimeMap.join _ ?s)] =>
+             apply TimeMap.join_r
+           | [|- TimeMap.le ?s (TimeMap.join ?s _)] =>
+             apply TimeMap.join_l
+           | [|- Memory.closed_capability Capability.bot ?m] =>
+             apply Memory.closed_capability_bot
+           | [|- Memory.closed_timemap TimeMap.bot ?m] =>
+             apply Memory.closed_timemap_bot
 
-           | [|- Capability.le (Capability.join_if _ _ _) _] =>
-             apply Capability.join_if_spec
-           | [|- Capability.le _ (if _ then _ else _)] =>
-             apply Capability.join_if_le
+           | [|- Capability.le (Capability.join _ _) _] =>
+             apply Capability.join_spec
+           | [|- Capability.le (Capability.singleton_ur _ _) _] =>
+             apply Capability.singleton_ur_spec
+           | [|- Capability.le (Capability.singleton_rw _ _) _] =>
+             apply Capability.singleton_rw_spec
+           | [|- Capability.le (Capability.singleton_sc _ _) _] =>
+             apply Capability.singleton_sc_spec
+           | [|- TimeMap.le (TimeMap.singleton _ _) _] =>
+             apply TimeMap.singleton_spec
+           | [|- Time.le (TimeMap.join _ _ _) _] =>
+             apply Time.join_spec
 
-            | [|- Memory.closed_capability (Capability.incr_ur _ _ _) _] =>
-              eapply Memory.incr_ur_closed_capability; eauto
-            | [|- Memory.closed_capability (Capability.incr_rw _ _ _) _] =>
-              eapply Memory.incr_rw_closed_capability; eauto
-            | [|- Memory.closed_capability (Capability.join _ _) _] =>
-              eapply Memory.join_closed_capability; eauto
+           | [|- Memory.closed_capability (Capability.join _ _) _] =>
+             eapply Memory.join_closed_capability; eauto
+           | [|- Memory.closed_capability (Capability.singleton_ur _ _) _] =>
+             eapply Memory.singleton_ur_closed_capability; eauto
+           | [|- Memory.closed_capability (Capability.singleton_rw _ _) _] =>
+             eapply Memory.singleton_rw_closed_capability; eauto
+           | [|- Memory.closed_capability (Capability.singleton_sc _ _) _] =>
+             eapply Memory.singleton_sc_closed_capability; eauto
+           | [|- Memory.closed_timemap (TimeMap.join _ _) _] =>
+             eapply Memory.join_closed_timemap; eauto
+           | [|- Memory.closed_timemap (TimeMap.singleton _ _) _] =>
+             eapply Memory.singleton_closed_timemap; eauto
 
-            | [|- Time.le (TimeMap.join _ _ _) _] =>
-              apply Time.join_spec
+           | [|- Capability.wf (Capability.join _ _)] =>
+             eapply Capability.join_wf; eauto
+           | [|- Capability.wf (Capability.singleton_ur _ _)] =>
+             eapply Capability.singleton_ur_wf; eauto
+           | [|- Capability.wf (Capability.singleton_rw _ _)] =>
+             eapply Capability.singleton_rw_wf; eauto
+           | [|- Capability.wf (Capability.singleton_sc _ _)] =>
+             eapply Capability.singleton_sc_wf; eauto
+           | [|- Capability.wf Capability.bot] =>
+             apply Capability.bot_wf
+
            end; subst; ss; i).
 
-  Lemma wf_get
-        loc commit1 mem
-        (CLOSED: Commit.closed commit1 mem):
-    exists msg,
-      Memory.get loc (commit1.(Commit.cur).(Capability.rw) loc) mem = Some msg.
-  Proof.
-    inversion CLOSED. inv CUR.
-    specialize (RW loc). des. eauto.
-  Qed.
-
-  Lemma read_mon1
+  Lemma readable_mon
         commit1 commit2
         (LE: Commit.le commit1 commit2):
-    Commit.read commit2 <5= Commit.read commit1.
+    Commit.readable commit2 <4= Commit.readable commit1.
   Proof.
-    i. inv PR. econs; auto.
+    s. i. inv PR. econs.
     - etrans; [apply LE|]. auto.
     - etrans; [apply LE|]. auto.
-    - etrans; [apply LE|]. auto.
-  Qed.
-
-  Lemma write_mon1
-        commit1 commit2
-        (LE: Commit.le commit1 commit2):
-    Commit.write commit2 <5= Commit.write commit1.
-  Proof.
-    i. inv PR. econs; auto.
-    - etrans; [apply LE|]. auto.
-    - eapply TimeFacts.le_lt_lt; [apply LE|]. eauto.
-    - etrans; [apply LE|]. auto.
-    - i. specialize (RA H). des. splits; auto.
+    - i. specialize (SC H). des. splits; auto.
       etrans; [apply LE|]. auto.
   Qed.
 
-  Lemma read_fence_mon1
+  Lemma writable_mon
         commit1 commit2
         (LE: Commit.le commit1 commit2):
-    Commit.read_fence commit2 <2= Commit.read_fence commit1.
+    Commit.writable commit2 <4= Commit.writable commit1.
   Proof.
-    i. inv PR. econs; auto.
-    - etrans; [apply LE|]. auto.
-    - etrans; [apply LE|]. auto.
+    s. i. inv PR. econs.
+    - eapply TimeFacts.le_lt_lt; [apply LE|]. auto.
+    - i. specialize (SC H). des. splits; auto.
+      eapply TimeFacts.le_lt_lt; [apply LE|]. auto.
   Qed.
 
-  Lemma write_fence_mon1
-        commit1 commit2
-        (LE: Commit.le commit1 commit2):
-    Commit.write_fence commit2 <2= Commit.write_fence commit1.
-  Proof.
-    i. inv PR. econs; auto.
-    - etrans; [apply LE|]. auto.
-    - etrans; [apply LE|]. auto.
-  Qed.
-
-  Lemma read_mon2
-        loc ts released
-        ord2 ord3
-        commit1 commit2 commit3
-        (READ: Commit.read commit1 loc ts released ord2 commit2)
-        (ORD: Ordering.le ord3 ord2)
-        (LE: Commit.le commit2 commit3)
-        (WF: Commit.wf commit3):
-    Commit.read commit1 loc ts released ord3 commit3.
-  Proof.
-    inv READ. econs; eauto.
-    - etrans; [|apply LE]. auto.
-    - i. rewrite ACQ; auto.
-      + apply LE.
-      + etrans; eauto.
-    - i. apply RW1. etrans; eauto.
-    - etrans; [|apply LE]. auto.
-    - etrans; [|apply LE].
-      apply RA. etrans; eauto.
-  Qed.
-
-  Lemma write_mon2
-        loc ts released
-        ord2 ord3
-        commit1 commit2 commit3
-        (WRITE: Commit.write commit1 loc ts released ord2 commit2)
-        (ORD: Ordering.le ord3 ord2)
-        (LE: Commit.le commit2 commit3)
-        (WF: Commit.wf commit3):
-    Commit.write commit1 loc ts released ord3 commit3.
-  Proof.
-    inv WRITE. econs; auto.
-    - etrans; [|apply LE]. auto.
-    - etrans; [|apply LE]. auto.
-    - etrans; [|apply LE]. auto.
-    - i. apply RA. etrans; eauto.
-  Qed.
-
-  Lemma read_fence_mon2
-        ord2 ord3
-        commit1 commit2 commit3
-        (FENCE: Commit.read_fence commit1 ord2 commit2)
-        (ORD: Ordering.le ord3 ord2)
-        (LE: Commit.le commit2 commit3)
-        (WF: Commit.wf commit3):
-    Commit.read_fence commit1 ord3 commit3.
-  Proof.
-    inv FENCE. econs; auto.
-    - etrans; [|apply LE]. auto.
-    - etrans; [|apply LE].
-      apply RA. etrans; eauto.
-  Qed.
-
-  Lemma write_fence_mon2
-        ord2 ord3
-        commit1 commit2 commit3
-        (FENCE: Commit.write_fence commit1 ord2 commit2)
-        (ORD: Ordering.le ord3 ord2)
-        (LE: Commit.le commit2 commit3)
-        (WF: Commit.wf commit3):
-    Commit.write_fence commit1 ord3 commit3.
-  Proof.
-    inv FENCE. econs; auto.
-    - etrans; [|apply LE]. auto.
-    - etrans; [|apply LE]. apply RA. etrans; eauto.
-  Qed.
-
-  Definition read_min
-             loc ts released ord commit: Commit.t :=
-    (Commit.mk commit.(Commit.rel)
-               (Capability.join_if
-                  (Ordering.le Ordering.acqrel ord)
-                  released
-                  (Capability.incr_rw loc ts commit.(Commit.cur)))
-               (Capability.join_if
-                  (Ordering.le Ordering.relaxed ord)
-                  released
-                  (Capability.incr_rw loc ts commit.(Commit.acq)))).
-
-  Lemma read_min_spec
-        loc ts released ord commit
-        (UR: Time.le (commit.(Commit.cur).(Capability.ur) loc) ts)
-        (RW: Ordering.le Ordering.relaxed ord -> Time.le (commit.(Commit.cur).(Capability.rw) loc) ts)
-        (WF1: Commit.wf commit)
-        (WF_RELEASED: Capability.wf released):
-    Commit.read commit loc ts released ord (read_min loc ts released ord commit).
-  Proof.
-    unfold read_min. econs; tac.
-    - econs; tac; try refl.
-      + unfold Capability.join_if. condtac; tac.
-        rewrite <- Capability.join_r. tac.
-      + unfold Capability.join_if. condtac; tac.
-        rewrite <- Capability.join_r. tac.
-    - unfold Capability.join_if. condtac; tac.
-    - unfold Capability.join_if. condtac; tac.
-      + etrans; [|apply TimeMap.join_r].
-        apply TimeMap.incr_ts.
-      + apply TimeMap.incr_ts.
-    - rewrite H. s. apply Capability.join_l.
-    - econs; s.
-      + apply WF1.
-      + apply Capability.join_if_wf; auto.
-        apply Capability.incr_rw_wf; auto.
-        apply WF1.
-      + apply Capability.join_if_wf; auto.
-        apply Capability.incr_rw_wf; auto.
-        apply WF1.
-      + i. unfold Capability.join_if. condtac; tac.
-        * etrans; [apply WF1|].
-          rewrite <- Capability.join_r. tac.
-        * etrans; [apply WF1|]. tac.
-      + unfold Capability.join_if.
-        repeat condtac; (try by destruct ord; inv COND0; inv COND); tac.
-        * etrans; [apply WF1|].
-          rewrite <- Capability.join_r. tac.
-        * etrans; [|apply Time.join_r].
-          apply TimeMap.incr_ts.
-        * etrans; [|apply Time.join_r].
-          apply TimeMap.incr_ts.
-        * etrans; [apply WF1|].
-          rewrite <- Capability.join_r. tac.
-        * etrans; [|apply Time.join_r].
-          apply TimeMap.incr_ts.
-        * etrans; [|apply Time.join_r].
-          apply TimeMap.incr_ts.
-        * etrans; [apply WF1|].
-          apply Capability.incr_rw_le.
-        * apply TimeMap.incr_ts.
-        * apply TimeMap.incr_ts.
-  Qed.
-
-  Lemma read_min_closed
-        loc from to val released ord commit mem
-        (MEM: Memory.closed mem)
-        (COMMIT: Commit.closed commit mem)
-        (GET: Memory.get loc to mem = Some (from, Message.mk val released))
-        (READ: Commit.read commit loc to released ord (read_min loc to released ord commit)):
-    Commit.closed (read_min loc to released ord commit) mem.
-  Proof.
-    inv MEM. exploit CLOSED; eauto. i. des.
-    econs; s.
-    - apply COMMIT.
-    - unfold Capability.join_if. condtac; tac.
-      + apply COMMIT.
-      + apply COMMIT.
-    - unfold Capability.join_if. condtac; tac.
-      + apply COMMIT.
-      + apply COMMIT.
-  Qed.
-
-  Lemma read_min_min
-        loc ts released ord commit1 commit2
-        (COMMIT2: Commit.read commit1 loc ts released ord commit2):
-    Commit.le (read_min loc ts released ord commit1) commit2.
-  Proof.
-    inv COMMIT2. unfold read_min. econs; tac.
-    - apply MON.
-    - apply MON.
-    - rewrite RW2. apply WF.
-    - apply MON.
-    - etrans; eauto. apply WF.
-    - etrans; eauto. etrans; apply WF.
-  Qed.
-
-  Definition write_min
-             loc ts released commit: Commit.t :=
-    (Commit.mk (LocFun.add loc released commit.(Commit.rel))
-               (Capability.join released (Capability.incr_ur loc ts commit.(Commit.cur)))
-               (Capability.join released (Capability.incr_ur loc ts commit.(Commit.acq)))).
-
-  Lemma write_min_spec
-        loc ts released ord commit
-        (RELEASED: Time.le (released.(Capability.rw) loc) ts)
-        (RW1: Time.lt (commit.(Commit.cur).(Capability.rw) loc) ts)
-        (REL1: Capability.le (commit.(Commit.rel) loc) released)
-        (RA: Ordering.le Ordering.acqrel ord ->
-             Capability.le commit.(Commit.cur) released /\
-             Time.le ts (released.(Capability.rw) loc))
-        (WF1: Commit.wf commit)
-        (WF_RELEASED: Capability.wf released):
-    Commit.write commit loc ts released ord (write_min loc ts released commit).
+  Lemma read_commit_incr
+        commit1 loc ts released ord:
+    Commit.le commit1 (Commit.read_commit commit1 loc ts released ord).
   Proof.
     econs; tac.
-    - econs; tac.
-      + unfold LocFun.add, LocFun.find. condtac; tac. refl.
-      + rewrite <- Capability.join_r. tac.
-      + rewrite <- Capability.join_r. tac.
-    - etrans; [|apply TimeMap.join_r].
-      apply TimeMap.incr_ts.
-    - unfold LocFun.add, LocFun.find.
-      condtac; [|congr]. refl.
-    - econs; try apply WF1; tac.
-      + unfold LocFun.add, LocFun.find. condtac; auto. apply WF1.
-      + apply Capability.join_wf; auto.
-        apply Capability.incr_ur_wf. apply WF1.
-      + apply Capability.join_wf; auto.
-        apply Capability.incr_ur_wf. apply WF1.
-      + unfold LocFun.add, LocFun.find. condtac; tac.
-        rewrite <- Capability.join_r.
-        rewrite <- Capability.incr_ur_le.
-        apply WF1.
-      + rewrite <- Capability.join_r.
-        rewrite <- Capability.incr_ur_le.
-        apply WF1.
-      + etrans; [|apply TimeMap.join_r].
-        apply TimeMap.incr_ts.
-      + etrans; [|apply TimeMap.join_r].
-        apply TimeMap.incr_ts.
-      + etrans; [|apply TimeMap.join_r].
-        apply TimeMap.incr_ts.
+    - rewrite <- ? Capability.join_l. refl.
+    - rewrite <- ? Capability.join_l. refl.
   Qed.
 
-  Lemma write_min_closed
-        loc from to val releasedc releasedm ord commit mem
+  Lemma write_commit_incr
+        commit1 sc1 loc ts ord:
+    Commit.le commit1 (Commit.write_commit commit1 sc1 loc ts ord).
+  Proof.
+    econs; tac.
+    - rewrite LocFun.add_spec. condtac; tac.
+      subst. rewrite <- Capability.join_l. refl.
+    - rewrite <- ? Capability.join_l. refl.
+    - rewrite <- ? Capability.join_l. refl.
+  Qed.
+
+  Lemma write_sc_incr
+        sc1 loc ts ord:
+    TimeMap.le sc1 (Commit.write_sc sc1 loc ts ord).
+  Proof.
+    unfold Commit.write_sc. tac.
+  Qed.
+
+  Lemma read_fence_commit_incr
+        commit1 ord
+        (WF1: Commit.wf commit1):
+    Commit.le commit1 (Commit.read_fence_commit commit1 ord).
+  Proof.
+    econs; tac. condtac; tac. apply WF1.
+  Qed.
+
+  Lemma write_fence_commit_incr
+        commit1 sc1 ord:
+    Commit.le commit1 (Commit.write_fence_commit commit1 sc1 ord).
+  Proof.
+    econs; tac. unfold LocFun.find. repeat condtac; tac.
+  Qed.
+
+  Lemma write_fence_sc_incr
+        commit1 sc1 ord:
+    TimeMap.le sc1 (Commit.write_fence_sc commit1 sc1 ord).
+  Proof.
+    unfold Commit.write_fence_sc. condtac; tac.
+  Qed.
+
+  (* CHECK: monotonicity? min_spec? min_min? *)
+
+  Lemma read_future
+        loc from to val released ord commit mem
         (MEM: Memory.closed mem)
-        (COMMIT: Commit.closed commit mem)
-        (GET: Memory.get loc to mem = Some (from, Message.mk val releasedm))
-        (CLOSED: Memory.closed_capability releasedc mem)
-        (WRITE: Commit.write commit loc to releasedc ord (write_min loc to releasedc commit)):
-    Commit.closed (write_min loc to releasedc commit) mem.
+        (WF_COMMIT: Commit.wf commit)
+        (CLOSED_COMMIT: Commit.closed commit mem)
+        (RELEASED: Capability.wf released)
+        (GET: Memory.get loc to mem = Some (from, Message.mk val released)):
+    <<WF_COMMIT: Commit.wf (Commit.read_commit commit loc to released ord)>> /\
+    <<CLOSED_COMMIT: Commit.closed (Commit.read_commit commit loc to released ord) mem>>.
   Proof.
-    inv MEM. exploit CLOSED0; eauto. i. des.
-    econs; s.
-    - i. unfold LocFun.add. condtac; auto. apply COMMIT.
-    - tac. apply COMMIT.
-    - tac. apply COMMIT.
+    splits; tac.
+    - econs; repeat (try condtac; tac);
+      try by rewrite <- ? Capability.join_l; apply WF_COMMIT.
+      + apply TimeMap.singleton_inv.
+        rewrite <- TimeMap.join_l. tac.
+      + apply TimeMap.singleton_inv.
+        rewrite <- TimeMap.join_l. tac.
+      + destruct ord; inv COND; inv COND0.
+    - inv MEM. exploit CLOSED; eauto. i. des.
+      econs; tac; try apply CLOSED_COMMIT.
+      + condtac; tac.
+      + condtac; tac.
   Qed.
 
-  Lemma write_min_min
-        loc ts released ord commit1 commit2
-        (COMMIT2: Commit.write commit1 loc ts released ord commit2):
-    Commit.le (write_min loc ts released commit1) commit2.
+  Lemma write_future
+        loc from to val releasedm ord commit sc mem
+        (MEM: Memory.closed mem)
+        (WF_COMMIT: Commit.wf commit)
+        (CLOSED_COMMIT: Commit.closed commit mem)
+        (CLOSED_SC: Memory.closed_timemap sc mem)
+        (GET: Memory.get loc to mem = Some (from, Message.mk val releasedm)):
+    <<WF_COMMIT: Commit.wf (Commit.write_commit commit sc loc to ord)>> /\
+    <<CLOSED_COMMIT: Commit.closed (Commit.write_commit commit sc loc to ord) mem>> /\
+    <<CLOSED_SC: Memory.closed_timemap (Commit.write_sc sc loc to ord) mem>>.
   Proof.
-    i. inv COMMIT2.
-    econs; tac;
-      (try by apply MON);
-      (try by etrans; eauto; apply WF).
-    - unfold LocFun.add, LocFun.find. condtac; tac.
-      apply MON.
-    - rewrite RW2. inv WF. etrans; apply CUR.
-    - rewrite REL2. etrans; apply WF.
-    - rewrite RW2. etrans; apply WF.
-    - rewrite RW2. etrans; [apply WF|].
-      inv WF. etrans; apply ACQ.
+    splits; tac.
+    - econs; tac; try apply WF_COMMIT.
+      + unfold LocFun.add, LocFun.find. repeat condtac; tac; try apply WF_COMMIT.
+        econs; try apply TimeMap.bot_spec.
+      + condtac; tac; try apply WF_COMMIT.
+        econs; try apply TimeMap.bot_spec.
+      + condtac; tac. econs; apply TimeMap.bot_spec.
+      + unfold LocFun.add, LocFun.find.
+        repeat condtac; tac; rewrite <- ? Capability.join_l; apply WF_COMMIT.
+      + repeat condtac; tac; rewrite <- ? Capability.join_l; apply WF_COMMIT.
+      + condtac; tac. econs; apply TimeMap.bot_spec.
+      + apply TimeMap.singleton_inv. rewrite <- TimeMap.join_l. tac.
+    - econs; tac; try by apply CLOSED_COMMIT.
+      + unfold LocFun.add. repeat condtac; tac; try by apply CLOSED_COMMIT.
+        econs; tac.
+      + condtac; tac. econs; tac.
+      + condtac; tac. econs; tac.
+    - unfold Commit.write_sc. condtac; tac.
   Qed.
 
-  Definition read_fence_min
-             ord commit: Commit.t :=
-    Commit.mk commit.(Commit.rel)
-              (if Ordering.le Ordering.acqrel ord
-               then commit.(Commit.acq)
-               else commit.(Commit.cur))
-              commit.(Commit.acq).
-
-  Lemma read_fence_min_spec
-        ord commit
-        (WF1: Commit.wf commit):
-    Commit.read_fence commit ord (read_fence_min ord commit).
-  Proof.
-    unfold read_fence_min. econs; tac; try apply WF1.
-    - econs; tac; try refl. apply WF1.
-    - refl.
-    - econs; s; try apply WF1.
-      + condtac; try apply WF1.
-      + i. condtac; try apply WF1.
-        etrans; apply WF1.
-      + condtac; try apply WF1. refl.
-  Qed.
-
-  Lemma read_fence_min_closed
+  Lemma read_fence_future
         ord commit mem
-        (FENCE: Commit.read_fence commit ord (read_fence_min ord commit))
-        (COMMIT: Commit.closed commit mem):
-    Commit.closed (read_fence_min ord commit) mem.
+        (WF_COMMIT: Commit.wf commit)
+        (CLOSED_COMMIT: Commit.closed commit mem):
+    <<WF_COMMIT: Commit.wf (Commit.read_fence_commit commit ord)>> /\
+    <<CLOSED_COMMIT: Commit.closed (Commit.read_fence_commit commit ord) mem>>.
   Proof.
-    econs; s.
-    - apply COMMIT.
-    - condtac.
-      + apply COMMIT.
-      + apply COMMIT.
-    - apply COMMIT.
+    splits.
+    - econs; tac; try apply WF_COMMIT.
+      + condtac; try apply WF_COMMIT.
+      + condtac; try apply WF_COMMIT.
+        etrans; apply WF_COMMIT.
+      + condtac; try apply WF_COMMIT. refl.
+    - econs; tac; try apply CLOSED_COMMIT.
+      condtac; try apply CLOSED_COMMIT.
   Qed.
 
-  Lemma read_fence_min_min
-        ord commit1 commit2
-        (WF1: Commit.wf commit1)
-        (COMMIT2: Commit.read_fence commit1 ord commit2):
-    Commit.le (read_fence_min ord commit1) commit2.
+  Lemma write_fence_future
+        ord commit sc mem
+        (WF_COMMIT: Commit.wf commit)
+        (CLOSED_COMMIT: Commit.closed commit mem)
+        (CLOSED_SC: Memory.closed_timemap sc mem):
+    <<WF_COMMIT: Commit.wf (Commit.write_fence_commit commit sc ord)>> /\
+    <<CLOSED_COMMIT: Commit.closed (Commit.write_fence_commit commit sc ord) mem>> /\
+    <<CLOSED_SC: Memory.closed_timemap (Commit.write_fence_sc commit sc ord) mem>>.
   Proof.
-    inv COMMIT2. unfold read_fence_min. econs; tac; try apply MON.
-    condtac; try apply MON. eauto.
-  Qed.
-
-  Definition write_fence_min
-             ord commit: Commit.t :=
-    Commit.mk (fun loc =>
-                 if Ordering.le Ordering.acqrel ord
-                 then commit.(Commit.cur)
-                 else (commit.(Commit.rel) loc))
-              commit.(Commit.cur)
-              commit.(Commit.acq).
-
-  Lemma write_fence_min_spec
-        ord commit
-        (WF1: Commit.wf commit):
-    Commit.write_fence commit ord (write_fence_min ord commit).
-  Proof.
-    econs; tac; try refl.
-    - econs; tac; try refl.
-      condtac; try refl.
-      apply WF1.
-    - econs; tac; try apply WF1.
-      + condtac; apply WF1.
-      + condtac; try apply WF1. refl.
-  Qed.
-
-  Lemma write_fence_min_closed
-        ord commit mem
-        (FENCE: Commit.write_fence commit ord (write_fence_min ord commit))
-        (COMMIT: Commit.closed commit mem):
-    Commit.closed (write_fence_min ord commit) mem.
-  Proof.
-    econs; s.
-    - i. condtac.
-      + apply COMMIT.
-      + apply COMMIT.
-    - apply COMMIT.
-    - apply COMMIT.
-  Qed.
-
-  Lemma write_fence_min_min
-        ord commit1 commit2
-        (WF1: Commit.wf commit1)
-        (COMMIT2: Commit.write_fence commit1 ord commit2):
-    Commit.le (write_fence_min ord commit1) commit2.
-  Proof.
-    inv COMMIT2. unfold write_fence_min. econs; tac; try apply MON.
-    condtac; try apply MON. eauto.
+    splits; tac.
+    - econs; tac; try apply WF_COMMIT.
+      + repeat condtac; tac; try apply WF_COMMIT.
+        econs; tac.
+      + repeat condtac; tac; try apply WF_COMMIT.
+        econs; tac.
+      + repeat condtac; tac. econs; tac.
+      + repeat condtac; tac; rewrite <- Capability.join_l; apply WF_COMMIT.
+      + repeat condtac; tac.
+      + repeat condtac; tac; rewrite <- Capability.join_l; apply WF_COMMIT.
+    - econs; tac; try apply CLOSED_COMMIT.
+      + unfold Commit.write_fence_sc.
+        repeat condtac; tac; try apply CLOSED_COMMIT.
+        econs; tac; try apply CLOSED_COMMIT.
+      + unfold Commit.write_fence_sc.
+        repeat condtac; tac; try apply CLOSED_COMMIT.
+        econs; tac; try apply CLOSED_COMMIT.
+      + unfold Commit.write_fence_sc.
+        repeat condtac; tac; try apply CLOSED_COMMIT.
+        econs; tac; try apply CLOSED_COMMIT.
+    - unfold Commit.write_fence_sc.
+      condtac; tac; try apply CLOSED_COMMIT.
   Qed.
 End CommitFacts.
 
