src/lang/Thread.v
@@ -20,7 +20,6 @@ Set Implicit Arguments.
 Module ThreadEvent.
   Inductive t :=
   | promise (loc:Loc.t) (from to:Time.t) (val:Const.t) (released:Capability.t)
-  | strengthen (loc:Loc.t) (from to:Time.t) (val:Const.t) (released1 released2:Capability.t)
   | silent
   | read (loc:Loc.t) (ts:Time.t) (val:Const.t) (ord:Ordering.t)
   | write (loc:Loc.t) (ts:Time.t) (val:Const.t) (ord:Ordering.t)
@@ -57,7 +56,7 @@ Module Local.
     promises: Memory.t;
   }.
 
-  Definition init := mk Commit.elt Memory.bot.
+  Definition init := mk Commit.bot Memory.bot.
 
   Inductive is_terminal (lc:t): Prop :=
   | is_terminal_intro
@@ -91,16 +90,6 @@ Module Local.
       promise_step lc1 mem1 loc from to val released (mk commit2 promises2) mem2 kind
   .
 
-  Inductive strengthen_step (lc1:t) (mem1:Memory.t) (loc:Loc.t) (from to:Time.t) (val:Const.t) (released1 released2:Capability.t): forall (lc2:t) (mem2:Memory.t), Prop :=
-  | step_strengthen
-      commit2 promises2 mem2
-      (PROMISE: Memory.strengthen lc1.(promises) mem1 loc from to val released1 released2 promises2 mem2)
-      (COMMIT: Commit.le lc1.(commit) commit2)
-      (COMMIT_WF: Commit.wf commit2)
-      (COMMIT_CLOSED: Commit.closed commit2 mem2):
-      strengthen_step lc1 mem1 loc from to val released1 released2 (mk commit2 promises2) mem2
-  .
-
   Inductive silent_step (lc1:t) (mem1:Memory.t): forall (lc2:t), Prop :=
   | step_silent
       commit2
@@ -112,23 +101,21 @@ Module Local.
 
   Inductive read_step (lc1:t) (mem1:Memory.t) (loc:Loc.t) (to:Time.t) (val:Const.t) (released:Capability.t) (ord:Ordering.t): forall (lc2:t), Prop :=
   | step_read
-      from releasedm
+      from
       commit2
-      (GET: Memory.get loc to mem1 = Some (from, Message.mk val releasedm))
-      (RELEASED: Capability.le releasedm released)
-      (COMMIT: Commit.read lc1.(commit) loc to released ord commit2)
-      (COMMIT_CLOSED: Commit.closed commit2 mem1):
+      (GET: Memory.get loc to mem1 = Some (from, Message.mk val released))
+      (COMMIT: Commit.read_commit lc1.(commit) loc to released ord = commit2):
       read_step lc1 mem1 loc to val released ord (mk commit2 lc1.(promises))
   .
 
-  Inductive fulfill_step (lc1:t) (mem1:Memory.t) (loc:Loc.t) (from to:Time.t) (val:Const.t) (releasedc releasedm:Capability.t) (ord:Ordering.t): forall (lc2:t), Prop :=
+  Inductive fulfill_step (lc1:t) (sc1:TimeMap.t) (mem1:Memory.t) (loc:Loc.t) (from to:Time.t) (val:Const.t) (releasedm released:Capability.t) (ord:Ordering.t): forall (lc2:t) (sc2:TimeMap.t), Prop :=
   | step_fulfill
-      commit2 promises2
-      (FULFILL: Memory.fulfill lc1.(promises) loc from to val releasedm promises2)
-      (COMMIT: Commit.write lc1.(commit) loc to releasedc ord commit2)
-      (COMMIT_CLOSED: Commit.closed commit2 mem1)
-      (RELEASED_CLOSED: Memory.closed_capability releasedc mem1):
-      fulfill_step lc1 mem1 loc from to val releasedc releasedm ord (mk commit2 promises2)
+      promises2
+      (FULFILL: Memory.fulfill lc1.(promises) loc from to val released promises2)
+      (RELEASED: Capability.join releasedm ((Commit.write_commit lc1.(commit) sc1 loc to ord).(Commit.rel) loc) = released):
+      fulfill_step lc1 sc1 mem1 loc from to val releasedm released ord
+                   (mk (Commit.write_commit lc1.(commit) sc1 loc to ord) promises2)
+                   (Commit.write_sc sc1 loc to ord)
   .
 
   Inductive write_kind :=
@@ -136,153 +123,148 @@ Module Local.
   | write_kind_promise_fulfill
   .
 
-  Inductive write_step (lc1:t) (mem1:Memory.t) (loc:Loc.t) (from to:Time.t) (val:Const.t) (releasedc releasedm:Capability.t) (ord:Ordering.t): forall (lc2:t) (mem2:Memory.t) (kind:write_kind), Prop :=
+  Inductive write_step (lc1:t) (sc1:TimeMap.t) (mem1:Memory.t) (loc:Loc.t) (from to:Time.t) (val:Const.t) (releasedm released:Capability.t) (ord:Ordering.t): forall (lc2:t) (sc2:TimeMap.t) (mem2:Memory.t) (kind:write_kind), Prop :=
   | step_write_fulfill
-      lc2
-      (FULFILL: fulfill_step lc1 mem1 loc from to val releasedc releasedm ord lc2)
+      lc2 sc2
+      (FULFILL: fulfill_step lc1 sc1 mem1 loc from to val releasedm released ord lc2 sc2)
       (RELEASE: Ordering.le Ordering.acqrel ord -> lc1.(promises) loc = Cell.bot):
-      write_step lc1 mem1 loc from to val releasedc releasedm ord lc2 mem1 write_kind_fulfill
+      write_step lc1 sc1 mem1 loc from to val releasedm released ord lc2 sc2 mem1 write_kind_fulfill
   | step_write_promise_fulfill
-      lc2 mem2 lc3
-      (PROMISE: promise_step lc1 mem1 loc from to val releasedm lc2 mem2 Memory.promise_kind_add)
-      (FULFILL: fulfill_step lc2 mem2 loc from to val releasedc releasedm ord lc3)
+      lc2 mem2 lc3 sc3
+      (PROMISE: promise_step lc1 mem1 loc from to val released lc2 mem2 Memory.promise_kind_add)
+      (FULFILL: fulfill_step lc2 sc1 mem2 loc from to val releasedm released ord lc3 sc3)
       (RELEASE: Ordering.le Ordering.acqrel ord -> lc1.(promises) loc = Cell.bot):
-      write_step lc1 mem1 loc from to val releasedc releasedm ord lc3 mem2 write_kind_promise_fulfill
+      write_step lc1 sc1 mem1 loc from to val releasedm released ord lc3 sc3 mem2 write_kind_promise_fulfill
   .
 
-  Inductive fence_step (lc1:t) (mem1:Memory.t) (ordr ordw:Ordering.t): forall (lc2:t), Prop :=
+  Inductive fence_step (lc1:t) (sc1:TimeMap.t) (mem1:Memory.t) (ordr ordw:Ordering.t): forall (lc2:t) (sc2:TimeMap.t), Prop :=
   | step_fence
-      commit2 commit3
-      (READ: Commit.read_fence lc1.(commit) ordr commit2)
-      (WRITE: Commit.write_fence commit2 ordw commit3)
-      (RELEASE: Ordering.le Ordering.acqrel ordw -> lc1.(promises) = Memory.bot)
-      (COMMIT_CLOSED: Commit.closed commit3 mem1):
-      fence_step lc1 mem1 ordr ordw (mk commit3 lc1.(promises))
+      commit2
+      (READ: Commit.read_fence_commit lc1.(commit) ordr = commit2)
+      (RELEASE: Ordering.le Ordering.acqrel ordw -> lc1.(promises) = Memory.bot):
+      fence_step lc1 sc1 mem1 ordr ordw (mk (Commit.write_fence_commit commit2 sc1 ordw) lc1.(promises)) (Commit.write_fence_sc commit2 sc1 ordw)
   .
 
-  Lemma future_read_step lc1 mem1 mem1' loc ts val released ord lc2
-        (FUTURE: Memory.future mem1 mem1')
-        (STEP: read_step lc1 mem1 loc ts val released ord lc2):
-    read_step lc1 mem1' loc ts val released ord lc2.
-  Proof.
-    inv STEP. exploit Memory.future_get; eauto. i. des.
-    econs; eauto.
-    - etrans; eauto.
-    - eapply Commit.future_closed; eauto.
-  Qed.
+  (* Lemma future_read_step lc1 mem1 mem1' loc ts val released ord lc2 *)
+  (*       (FUTURE: Memory.future mem1 mem1') *)
+  (*       (STEP: read_step lc1 mem1 loc ts val released ord lc2): *)
+  (*   read_step lc1 mem1' loc ts val released ord lc2. *)
+  (* Proof. *)
+  (*   inv STEP. exploit Memory.future_get; eauto. i. des. *)
+  (*   econs; eauto. *)
+  (* Qed. *)
 
-  Lemma future_fulfill_step lc1 mem1 mem1' loc from to val releasedc releasedm ord lc2
+  Lemma future_fulfill_step lc1 sc1 mem1 mem1' loc from to val releasedm released ord lc2 sc2
         (FUTURE: Memory.future mem1 mem1')
-        (STEP: fulfill_step lc1 mem1 loc from to val releasedc releasedm ord lc2):
-    fulfill_step lc1 mem1' loc from to val releasedc releasedm ord lc2.
+        (STEP: fulfill_step lc1 sc1 mem1 loc from to val releasedm released ord lc2 sc2):
+    fulfill_step lc1 sc1 mem1' loc from to val releasedm released ord lc2 sc2.
   Proof.
     inv STEP. econs; eauto.
-    - eapply Commit.future_closed; eauto.
-    - eapply Memory.future_closed_capability; eauto.
   Qed.
 
-  Lemma future_fence_step lc1 mem1 mem1' ordr ordw lc2
+  Lemma future_fence_step lc1 sc1 mem1 mem1' ordr ordw lc2 sc2
         (FUTURE: Memory.future mem1 mem1')
-        (STEP: fence_step lc1 mem1 ordr ordw lc2):
-    fence_step lc1 mem1' ordr ordw lc2.
+        (STEP: fence_step lc1 sc1 mem1 ordr ordw lc2 sc2):
+    fence_step lc1 sc1 mem1' ordr ordw lc2 sc2.
   Proof.
     inv STEP. econs; eauto.
-    eapply Commit.future_closed; eauto.
   Qed.
 
-  Lemma read_step_mon2
-        lc1 mem1 loc to val released ord ord' lc2
-        (READ: read_step lc1 mem1 loc to val released ord lc2)
-        (ORD: Ordering.le ord' ord):
-    read_step lc1 mem1 loc to val released ord' lc2.
-  Proof.
-    inv READ. econs; eauto. eapply CommitFacts.read_mon2; eauto.
-    - refl.
-    - apply COMMIT.
-  Qed.
-
-  Lemma promise_step_future lc1 mem1 loc from to val released lc2 mem2 kind
+  Lemma promise_step_future lc1 sc1 mem1 loc from to val released lc2 mem2 kind
         (STEP: promise_step lc1 mem1 loc from to val released lc2 mem2 kind)
         (WF1: wf lc1 mem1)
+        (SC1: Memory.closed_timemap sc1 mem1)
         (CLOSED1: Memory.closed mem1):
     <<WF2: wf lc2 mem2>> /\
+    <<SC2: Memory.closed_timemap sc1 mem2>> /\
     <<CLOSED2: Memory.closed mem2>> /\
     <<FUTURE: Memory.future mem1 mem2>>.
   Proof.
     inv WF1. inv STEP.
     exploit Memory.promise_future; eauto. i. des.
-    splits; ss.
+    splits; ss. eapply Memory.future_closed_timemap; eauto.
   Qed.
 
-  Lemma strengthen_step_future lc1 mem1 loc from to val released1 released2 lc2 mem2
-        (STEP: strengthen_step lc1 mem1 loc from to val released1 released2 lc2 mem2)
-        (WF1: wf lc1 mem1)
-        (CLOSED1: Memory.closed mem1):
-    <<WF2: wf lc2 mem2>> /\
-    <<CLOSED2: Memory.closed mem2>> /\
-    <<FUTURE: Memory.future mem1 mem2>>.
-  Proof.
-    inv WF1. inv STEP.
-    exploit Memory.strengthen_future; eauto. i. des.
-    splits; ss.
-  Qed.
-
-  Lemma silent_step_future lc1 mem1 lc2
+  Lemma silent_step_future lc1 sc1 mem1 lc2
         (STEP: silent_step lc1 mem1 lc2)
         (WF1: wf lc1 mem1)
+        (SC1: Memory.closed_timemap sc1 mem1)
         (CLOSED1: Memory.closed mem1):
     wf lc2 mem1.
   Proof.
     inv WF1. inv STEP. ss.
   Qed.
 
-  Lemma read_step_future lc1 mem1 loc ts val released ord lc2
+  Lemma read_step_future lc1 sc1 mem1 loc ts val released ord lc2
         (STEP: read_step lc1 mem1 loc ts val released ord lc2)
         (WF1: wf lc1 mem1)
+        (SC1: Memory.closed_timemap sc1 mem1)
         (CLOSED1: Memory.closed mem1):
     wf lc2 mem1.
   Proof.
-    inv WF1. inv STEP. econs; ss. apply COMMIT.
+    inv WF1. inv STEP.
+    exploit CommitFacts.read_future; eauto.
+    { eapply CLOSED1. eauto. }
+    i. des. econs; eauto.
   Qed.
 
-  Lemma fulfill_step_future lc1 mem1 loc from to val releasedc releasedm ord lc2
-        (STEP: fulfill_step lc1 mem1 loc from to val releasedc releasedm ord lc2)
+  Lemma fulfill_step_future lc1 sc1 mem1 loc from to val releasedm released ord lc2 sc2
+        (STEP: fulfill_step lc1 sc1 mem1 loc from to val releasedm released ord lc2 sc2)
         (WF1: wf lc1 mem1)
+        (SC1: Memory.closed_timemap sc1 mem1)
         (CLOSED1: Memory.closed mem1):
-    wf lc2 mem1.
+    <<WF2: wf lc2 mem1>> /\
+    <<SC2: Memory.closed_timemap sc2 mem1>> /\
+    <<SC_FUTURE: TimeMap.le sc1 sc2>>.
   Proof.
-    inv WF1. inv STEP. econs; ss.
-    - apply COMMIT.
-    - eapply Memory.fulfill_future; eauto.
+    inv WF1. inv STEP.
+    exploit CommitFacts.write_future; eauto.
+    { apply PROMISES. eapply Memory.remove_disjoint. apply FULFILL. }
+    i. des. splits; eauto.
+    - econs; eauto.
+      s. eapply Memory.fulfill_future; eauto.
+    - apply CommitFacts.write_sc_incr.
   Qed.
 
-  Lemma write_step_future lc1 mem1 loc from to val releasedc releasedm ord lc2 mem2 kind
-        (STEP: write_step lc1 mem1 loc from to val releasedc releasedm ord lc2 mem2 kind)
+  Lemma write_step_future lc1 sc1 mem1 loc from to val releasedm released ord lc2 sc2 mem2 kind
+        (STEP: write_step lc1 sc1 mem1 loc from to val releasedm released ord lc2 sc2 mem2 kind)
         (WF1: wf lc1 mem1)
+        (SC1: Memory.closed_timemap sc1 mem1)
         (CLOSED1: Memory.closed mem1):
     <<WF2: wf lc2 mem2>> /\
+    <<SC2: Memory.closed_timemap sc2 mem2>> /\
     <<CLOSED2: Memory.closed mem2>> /\
-    <<FUTURE: Memory.future mem1 mem2>>.
+    <<SC_FUTURE: TimeMap.le sc1 sc2>> /\
+    <<MEM_FUTURE: Memory.future mem1 mem2>>.
   Proof.
     inv STEP.
-    - exploit fulfill_step_future; eauto. i. splits; ss. refl.
+    - exploit fulfill_step_future; eauto. i. des. splits; ss. refl.
     - exploit promise_step_future; eauto. i. des.
-      exploit fulfill_step_future; eauto.
+      exploit fulfill_step_future; eauto. i. des. auto.
   Qed.
 
-  Lemma fence_step_future lc1 mem1 ordr ordw lc2
-        (STEP: fence_step lc1 mem1 ordr ordw lc2)
+  Lemma fence_step_future lc1 sc1 mem1 ordr ordw lc2 sc2
+        (STEP: fence_step lc1 sc1 mem1 ordr ordw lc2 sc2)
         (WF1: wf lc1 mem1)
+        (SC1: Memory.closed_timemap sc1 mem1)
         (CLOSED1: Memory.closed mem1):
-    wf lc2 mem1.
+    <<WF2: wf lc2 mem1>> /\
+    <<SC2: Memory.closed_timemap sc2 mem1>> /\
+    <<SC_FUTURE: TimeMap.le sc1 sc2>>.
   Proof.
-    inv WF1. inv STEP. econs; ss. apply WRITE.
+    inv WF1. inv STEP.
+    exploit CommitFacts.read_fence_future; eauto. i. des.
+    exploit CommitFacts.write_fence_future; eauto. i. des.
+    splits; eauto.
+    - econs; eauto.
+    - apply CommitFacts.write_fence_sc_incr.
   Qed.
 
   Lemma promise_step_disjoint
-        lc1 mem1 loc from to val released lc2 mem2 lc kind
+        lc1 sc1 mem1 loc from to val released lc2 mem2 lc kind
         (STEP: promise_step lc1 mem1 loc from to val released lc2 mem2 kind)
         (WF1: wf lc1 mem1)
+        (SC1: Memory.closed_timemap sc1 mem1)
         (CLOSED1: Memory.closed mem1)
         (DISJOINT1: disjoint lc1 lc)
         (WF: wf lc mem1):
@@ -292,29 +274,15 @@ Module Local.
     inv WF1. inv DISJOINT1. inversion WF. inv STEP.
     exploit Memory.promise_future; try apply PROMISE; eauto. i. des.
     exploit Memory.promise_disjoint; try apply PROMISE; eauto. i. des.
-    splits; ss. econs; eauto. eapply Commit.future_closed; eauto.
-  Qed.
-
-  Lemma strengthen_step_disjoint
-        lc1 mem1 loc from to val released1 released2 lc2 mem2 lc
-        (STEP: strengthen_step lc1 mem1 loc from to val released1 released2 lc2 mem2)
-        (WF1: wf lc1 mem1)
-        (CLOSED1: Memory.closed mem1)
-        (DISJOINT1: disjoint lc1 lc)
-        (WF: wf lc mem1):
-    <<DISJOINT2: disjoint lc2 lc>> /\
-    <<WF: wf lc mem2>>.
-  Proof.
-    inv WF1. inv DISJOINT1. inversion WF. inv STEP.
-    exploit Memory.strengthen_future; try apply PROMISE; eauto. i. des.
-    exploit Memory.strengthen_disjoint; try apply PROMISE; eauto. i. des.
-    splits; ss. econs; eauto. eapply Commit.future_closed; eauto.
+    splits; ss. econs; eauto.
+    eapply Commit.future_closed; eauto.
   Qed.
 
   Lemma silent_step_disjoint
-        lc1 mem1 lc2 lc
+        lc1 sc1 mem1 lc2 lc
         (STEP: silent_step lc1 mem1 lc2)
         (WF1: wf lc1 mem1)
+        (SC1: Memory.closed_timemap sc1 mem1)
         (DISJOINT1: disjoint lc1 lc)
         (WF: wf lc mem1):
     disjoint lc2 lc.
@@ -323,9 +291,10 @@ Module Local.
   Qed.
 
   Lemma read_step_disjoint
-        lc1 mem1 lc2 loc ts val released ord lc
+        lc1 sc1 mem1 lc2 loc ts val released ord lc
         (STEP: read_step lc1 mem1 loc ts val released ord lc2)
         (WF1: wf lc1 mem1)
+        (SC1: Memory.closed_timemap sc1 mem1)
         (DISJOINT1: disjoint lc1 lc)
         (WF: wf lc mem1):
     disjoint lc2 lc.
@@ -334,9 +303,10 @@ Module Local.
   Qed.
 
   Lemma fulfill_step_disjoint
-        lc1 mem1 lc2 loc from to val releasedc releasedm ord lc
-        (STEP: fulfill_step lc1 mem1 loc from to val releasedc releasedm ord lc2)
+        lc1 sc1 mem1 lc2 sc2 loc from to val releasedm released ord lc
+        (STEP: fulfill_step lc1 sc1 mem1 loc from to val releasedm released ord lc2 sc2)
         (WF1: wf lc1 mem1)
+        (SC1: Memory.closed_timemap sc1 mem1)
         (CLOSED1: Memory.closed mem1)
         (DISJOINT1: disjoint lc1 lc)
         (WF: wf lc mem1):
@@ -349,9 +319,10 @@ Module Local.
   Qed.
 
   Lemma write_step_disjoint
-        lc1 mem1 lc2 loc from to val releasedc releasedm ord mem2 lc kind
-        (STEP: write_step lc1 mem1 loc from to val releasedc releasedm ord lc2 mem2 kind)
+        lc1 sc1 mem1 lc2 sc2 loc from to val releasedm released ord mem2 lc kind
+        (STEP: write_step lc1 sc1 mem1 loc from to val releasedm released ord lc2 sc2 mem2 kind)
         (WF1: wf lc1 mem1)
+        (SC1: Memory.closed_timemap sc1 mem1)
         (CLOSED1: Memory.closed mem1)
         (DISJOINT1: disjoint lc1 lc)
         (WF: wf lc mem1):
@@ -363,18 +334,21 @@ Module Local.
       exploit fulfill_step_disjoint; eauto.
     - exploit promise_step_future; eauto. i. des.
       exploit promise_step_disjoint; eauto. i. des.
+      exploit fulfill_step_future; eauto. i.
       exploit fulfill_step_disjoint; eauto.
   Qed.
 
   Lemma fence_step_disjoint
-        lc1 mem1 lc2 ordr ordw lc
-        (STEP: fence_step lc1 mem1 ordr ordw lc2)
+        lc1 sc1 mem1 lc2 sc2 ordr ordw lc
+        (STEP: fence_step lc1 sc1 mem1 ordr ordw lc2 sc2)
         (WF1: wf lc1 mem1)
+        (SC1: Memory.closed_timemap sc1 mem1)
         (DISJOINT1: disjoint lc1 lc)
         (WF: wf lc mem1):
-    disjoint lc2 lc.
+    <<DISJOINT2: disjoint lc2 lc>> /\
+    <<WF: wf lc mem1>>.
   Proof.
-    inv WF1. inv DISJOINT1. inv WF. inv STEP. ss.
+    inv WF1. inv DISJOINT1. inv WF. inv STEP. splits; ss.
   Qed.
 End Local.
 
@@ -385,22 +359,17 @@ Module Thread.
     Structure t := mk {
       state: lang.(Language.state);
       local: Local.t;
+      sc: TimeMap.t;
       memory: Memory.t;
     }.
 
-    Inductive memory_step: forall (e:ThreadEvent.t) (e1 e2:t), Prop :=
-    | step_promise
-        st lc1 mem1
+    Inductive promise_step: forall (e:ThreadEvent.t) (e1 e2:t), Prop :=
+    | promise_promise_intro
+        st lc1 sc1 mem1
         loc from to val released kind
         lc2 mem2
         (LOCAL: Local.promise_step lc1 mem1 loc from to val released lc2 mem2 kind):
-        memory_step (ThreadEvent.promise loc from to val released) (mk st lc1 mem1) (mk st lc2 mem2)
-    | step_strengthen
-        st lc1 mem1
-        loc from to val released1 released2
-        lc2 mem2
-        (LOCAL: Local.strengthen_step lc1 mem1 loc from to val released1 released2 lc2 mem2):
-        memory_step (ThreadEvent.strengthen loc from to val released1 released2) (mk st lc1 mem1) (mk st lc2 mem2)
+        promise_step (ThreadEvent.promise loc from to val released) (mk st lc1 sc1 mem1) (mk st lc2 sc1 mem2)
     .
 
     (* NOTE: Syscalls act like a write SC fence.  We did not let
@@ -414,49 +383,49 @@ Module Thread.
      *)
     Inductive program_step: forall (e:ThreadEvent.t) (e1 e2:t), Prop :=
     | step_silent
-        st1 lc1 mem1
+        st1 lc1 sc1 mem1
         st2 lc2
         (STATE: lang.(Language.step) None st1 st2)
         (LOCAL: Local.silent_step lc1 mem1 lc2):
-        program_step ThreadEvent.silent (mk st1 lc1 mem1) (mk st2 lc2 mem1)
+        program_step ThreadEvent.silent (mk st1 lc1 sc1 mem1) (mk st2 lc2 sc1 mem1)
     | step_read
-        st1 lc1 mem1
+        st1 lc1 sc1 mem1
         st2 loc ts val released ord lc2
         (STATE: lang.(Language.step) (Some (ProgramEvent.read loc val ord)) st1 st2)
         (LOCAL: Local.read_step lc1 mem1 loc ts val released ord lc2):
-        program_step (ThreadEvent.read loc ts val ord) (mk st1 lc1 mem1) (mk st2 lc2 mem1)
+        program_step (ThreadEvent.read loc ts val ord) (mk st1 lc1 sc1 mem1) (mk st2 lc2 sc1 mem1)
     | step_write
-        st1 lc1 mem1
-        st2 loc from to val released ord lc2 mem2 kind
+        st1 lc1 sc1 mem1
+        st2 loc from to val released ord lc2 sc2 mem2 kind
         (STATE: lang.(Language.step) (Some (ProgramEvent.write loc val ord)) st1 st2)
-        (LOCAL: Local.write_step lc1 mem1 loc from to val released released ord lc2 mem2 kind):
-        program_step (ThreadEvent.write loc to val ord) (mk st1 lc1 mem1) (mk st2 lc2 mem2)
+        (LOCAL: Local.write_step lc1 sc1 mem1 loc from to val Capability.bot released ord lc2 sc2 mem2 kind):
+        program_step (ThreadEvent.write loc to val ord) (mk st1 lc1 sc1 mem1) (mk st2 lc2 sc2 mem2)
     | step_update
-        st1 lc1 mem1
+        st1 lc1 sc1 mem1
         st3 loc ordr ordw
         tsr valr releasedr lc2
-        tsw valw releasedw lc3 mem3 kind
+        tsw valw releasedw lc3 sc3 mem3 kind
         (STATE: lang.(Language.step) (Some (ProgramEvent.update loc valr valw ordr ordw)) st1 st3)
         (LOCAL1: Local.read_step lc1 mem1 loc tsr valr releasedr ordr lc2)
-        (LOCAL2: Local.write_step lc2 mem1 loc tsr tsw valw releasedw (Capability.join releasedr releasedw) ordw lc3 mem3 kind):
-        program_step (ThreadEvent.update loc tsr tsw valr valw ordr ordw) (mk st1 lc1 mem1) (mk st3 lc3 mem3)
+        (LOCAL2: Local.write_step lc2 sc1 mem1 loc tsr tsw valw releasedr releasedw ordw lc3 sc3 mem3 kind):
+        program_step (ThreadEvent.update loc tsr tsw valr valw ordr ordw) (mk st1 lc1 sc1 mem1) (mk st3 lc3 sc3 mem3)
     | step_fence
-        st1 lc1 mem1
-        st2 ordr ordw lc2
+        st1 lc1 sc1 mem1
+        st2 ordr ordw lc2 sc2
         (STATE: lang.(Language.step) (Some (ProgramEvent.fence ordr ordw)) st1 st2)
-        (LOCAL: Local.fence_step lc1 mem1 ordr ordw lc2):
-        program_step (ThreadEvent.fence ordr ordw) (mk st1 lc1 mem1) (mk st2 lc2 mem1)
+        (LOCAL: Local.fence_step lc1 sc1 mem1 ordr ordw lc2 sc2):
+        program_step (ThreadEvent.fence ordr ordw) (mk st1 lc1 sc1 mem1) (mk st2 lc2 sc2 mem1)
     | step_syscall
-        st1 lc1 mem1
-        st2 e lc2
+        st1 lc1 sc1 mem1
+        st2 e lc2 sc2
         (STATE: lang.(Language.step) (Some (ProgramEvent.syscall e)) st1 st2)
-        (LOCAL: Local.fence_step lc1 mem1 Ordering.unordered Ordering.seqcst lc2):
-        program_step (ThreadEvent.syscall e) (mk st1 lc1 mem1) (mk st2 lc2 mem1)
+        (LOCAL: Local.fence_step lc1 sc1 mem1 Ordering.unordered Ordering.seqcst lc2 sc2):
+        program_step (ThreadEvent.syscall e) (mk st1 lc1 sc1 mem1) (mk st2 lc2 sc2 mem1)
     .
 
     Inductive step (e:ThreadEvent.t) (e1 e2:t): Prop :=
-    | step_memory
-        (STEP: memory_step e e1 e2)
+    | step_promise
+        (STEP: promise_step e e1 e2)
     | step_program
         (STEP: program_step e e1 e2)
     .
@@ -469,81 +438,94 @@ Module Thread.
     .
 
     Definition consistent (e:t): Prop :=
-      forall mem1
+      forall sc1 mem1
         (FUTURE: Memory.future e.(memory) mem1)
+        (FUTURE: TimeMap.le e.(sc) sc1)
         (WF: Local.wf e.(local) mem1)
+        (SC: Memory.closed_timemap sc1 mem1)
         (MEM: Memory.closed mem1),
       exists e2,
-        <<STEPS: rtc tau_step (mk e.(state) e.(local) mem1) e2>> /\
+        <<STEPS: rtc tau_step (mk e.(state) e.(local) sc1 mem1) e2>> /\
         <<PROMISES: e2.(local).(Local.promises) = Memory.bot>>.
 
-    Lemma memory_step_future
-          e  e1 e2
-          (STEP: memory_step e e1 e2)
+    Lemma promise_step_future
+          e e1 e2
+          (STEP: promise_step e e1 e2)
           (WF1: Local.wf e1.(local) e1.(memory))
+          (SC1: Memory.closed_timemap e1.(sc) e1.(memory))
           (CLOSED1: Memory.closed e1.(memory)):
       <<WF2: Local.wf e2.(local) e2.(memory)>> /\
+      <<SC2: Memory.closed_timemap e2.(sc) e2.(memory)>> /\
       <<CLOSED2: Memory.closed e2.(memory)>> /\
       <<FUTURE: Memory.future e1.(memory) e2.(memory)>>.
     Proof.
       inv WF1. inv STEP. s.
-      - exploit Local.promise_step_future; eauto. i. des.
-        splits; eauto. econs; eauto.
-      - exploit Local.strengthen_step_future; eauto. i. des.
-        splits; eauto. econs; eauto.
+      exploit Local.promise_step_future; eauto. i. des.
+      splits; eauto. econs; eauto.
     Qed.
 
     Lemma program_step_future e e1 e2
           (STEP: program_step e e1 e2)
           (WF1: Local.wf e1.(local) e1.(memory))
+          (SC1: Memory.closed_timemap e1.(sc) e1.(memory))
           (CLOSED1: Memory.closed e1.(memory)):
       <<WF2: Local.wf e2.(local) e2.(memory)>> /\
+      <<SC2: Memory.closed_timemap e2.(sc) e2.(memory)>> /\
       <<CLOSED2: Memory.closed e2.(memory)>> /\
-      <<FUTURE: Memory.future e1.(memory) e2.(memory)>>.
+      <<SC_FUTURE: TimeMap.le e1.(sc) e2.(sc)>> /\
+      <<MEM_FUTURE: Memory.future e1.(memory) e2.(memory)>>.
     Proof.
       inv STEP; ss.
-      - exploit Local.silent_step_future; eauto. i. splits; ss. refl.
-      - exploit Local.read_step_future; eauto. i. splits; ss. refl.
+      - exploit Local.silent_step_future; eauto. i. splits; ss; refl.
+      - exploit Local.read_step_future; eauto. i. splits; ss; refl.
       - exploit Local.write_step_future; eauto.
       - exploit Local.read_step_future; eauto. i.
         exploit Local.write_step_future; eauto.
-      - exploit Local.fence_step_future; eauto. i. splits; ss. refl.
-      - exploit Local.fence_step_future; eauto. i. splits; ss. refl.
+      - exploit Local.fence_step_future; eauto. i. des. splits; ss. refl.
+      - exploit Local.fence_step_future; eauto. i. des. splits; ss. refl.
     Qed.
 
     Lemma step_future e e1 e2
           (STEP: step e e1 e2)
           (WF1: Local.wf e1.(local) e1.(memory))
+          (SC1: Memory.closed_timemap e1.(sc) e1.(memory))
           (CLOSED1: Memory.closed e1.(memory)):
       <<WF2: Local.wf e2.(local) e2.(memory)>> /\
+      <<SC2: Memory.closed_timemap e2.(sc) e2.(memory)>> /\
       <<CLOSED2: Memory.closed e2.(memory)>> /\
-      <<FUTURE: Memory.future e1.(memory) e2.(memory)>>.
+      <<SC_FUTURE: TimeMap.le e1.(sc) e2.(sc)>> /\
+      <<MEM_FUTURE: Memory.future e1.(memory) e2.(memory)>>.
     Proof.
       inv STEP.
-      - eapply memory_step_future; eauto.
+      - exploit promise_step_future; eauto. i. des. splits; ss.
+        inv STEP0. ss. refl.
       - eapply program_step_future; eauto.
     Qed.
 
     Lemma rtc_step_future e1 e2
           (STEP: rtc tau_step e1 e2)
           (WF1: Local.wf e1.(local) e1.(memory))
+          (SC1: Memory.closed_timemap e1.(sc) e1.(memory))
           (CLOSED1: Memory.closed e1.(memory)):
       <<WF2: Local.wf e2.(local) e2.(memory)>> /\
+      <<SC2: Memory.closed_timemap e2.(sc) e2.(memory)>> /\
       <<CLOSED2: Memory.closed e2.(memory)>> /\
-      <<FUTURE: Memory.future e1.(memory) e2.(memory)>>.
+      <<SC_FUTURE: TimeMap.le e1.(sc) e2.(sc)>> /\
+      <<MEM_FUTURE: Memory.future e1.(memory) e2.(memory)>>.
     Proof.
       revert WF1. induction STEP.
-      - i. splits; ss. refl.
+      - i. splits; ss; refl.
       - i. inv H.
         exploit step_future; eauto. i. des.
         exploit IHSTEP; eauto. i. des.
-        splits; ss. etrans; eauto.
+        splits; ss; etrans; eauto.
     Qed.
 
-    Lemma memory_step_disjoint
+    Lemma promise_step_disjoint
           e e1 e2 lc
-        (STEP: memory_step e e1 e2)
+        (STEP: promise_step e e1 e2)
         (WF1: Local.wf e1.(local) e1.(memory))
+        (SC1: Memory.closed_timemap e1.(sc) e1.(memory))
         (CLOSED1: Memory.closed e1.(memory))
         (DISJOINT1: Local.disjoint e1.(local) lc)
         (WF: Local.wf lc e1.(memory)):
@@ -551,15 +533,14 @@ Module Thread.
       <<WF: Local.wf lc e2.(memory)>>.
     Proof.
       inv STEP.
-      - exploit Local.promise_step_future; eauto. i. des.
-        exploit Local.promise_step_disjoint; eauto.
-      - exploit Local.strengthen_step_future; eauto. i. des.
-        exploit Local.strengthen_step_disjoint; eauto.
+      exploit Local.promise_step_future; eauto. i. des.
+      exploit Local.promise_step_disjoint; eauto.
     Qed.
 
     Lemma program_step_disjoint e e1 e2 lc
         (STEP: program_step e e1 e2)
         (WF1: Local.wf e1.(local) e1.(memory))
+        (SC1: Memory.closed_timemap e1.(sc) e1.(memory))
         (CLOSED1: Memory.closed e1.(memory))
         (DISJOINT1: Local.disjoint e1.(local) lc)
         (WF: Local.wf lc e1.(memory)):
@@ -586,6 +567,7 @@ Module Thread.
     Lemma step_disjoint e e1 e2 lc
         (STEP: step e e1 e2)
         (WF1: Local.wf e1.(local) e1.(memory))
+        (SC1: Memory.closed_timemap e1.(sc) e1.(memory))
         (CLOSED1: Memory.closed e1.(memory))
         (DISJOINT1: Local.disjoint e1.(local) lc)
         (WF: Local.wf lc e1.(memory)):
@@ -593,13 +575,14 @@ Module Thread.
       <<WF: Local.wf lc e2.(memory)>>.
     Proof.
       inv STEP.
-      - eapply memory_step_disjoint; eauto.
+      - eapply promise_step_disjoint; eauto.
       - eapply program_step_disjoint; eauto.
     Qed.
 
     Lemma rtc_step_disjoint e1 e2 lc
         (STEP: rtc tau_step e1 e2)
         (WF1: Local.wf e1.(local) e1.(memory))
+        (SC1: Memory.closed_timemap e1.(sc) e1.(memory))
         (CLOSED1: Memory.closed e1.(memory))
         (DISJOINT1: Local.disjoint e1.(local) lc)
         (WF: Local.wf lc e1.(memory)):
